checkpoint mail server progress from yesterday

src/FS/FSAPI.v
@@ -7,126 +7,10 @@ Require Import RelationClasses.
 Require Import Morphisms.
 Require Import Sumbool.
 Require Import FSModel.
+Require Import LinkAPI.
 
 Import ListNotations.
 Open Scope string.
-
-
-(** Opcodes *)
-
-Inductive linkOpT : Type -> Type :=
-| LinkAdd (dir : nat) (name : string) (target : Node) : linkOpT bool
-| LinkAllocFile (dir : nat) (name : string) : linkOpT (option nat)
-| LinkAllocDir (dir : nat) (name : string) : linkOpT (option nat)
-| LinkDel (dir : nat) (name : string) (target : Node) : linkOpT bool
-| LinkLookup (dir : nat) (name : string) : linkOpT (option Node)
-| LinkList (dir : nat) : linkOpT (option (list string))
-| LinkGetRoot : linkOpT nat
-| LinkFindUnusedName (dir : nat) (prefix : string) : linkOpT string
-| FileRead (f : nat) : linkOpT string
-| FileWrite (f : nat) (data : string) : linkOpT unit
-| GetTID : linkOpT nat.
-
-
-Inductive stat_result :=
-| StatFile
-| StatDir.
-
-(*
-Inductive fsOpT : Type -> Type :=
-| Create (cwd : nat) (dir : Pathname) (name : string) : fsOpT nat
-| Mkdir (cwd : nat) (dir : Pathname) (name : string) : fsOpT nat
-| Unlink (cwd : nat) (dir : Pathname) (name : string) : fsOpT unit
-| Stat (cwd : nat) (dir : Pathname) (name : string) : fsOpT (option stat_result)
-| Readdir (cwd : nat) (pn : Pathname) : fsOpT (list string)
-| Rename (cwd : nat) (src : Pathname) (dstdir : Pathname) (dstname : string) : fsOpT unit
-| Read (cwd : nat) (pn : Pathname) : fsOpT string
-| Write (cwd : nat) (pn : Pathname) (data : string) : fsOpT unit
-| FindAvailableName (cwd : nat) (dir : Pathname) : fsOpT string
-| Debug (s : string) : fsOpT unit.
-*)
-
-
-Module LinkAPI <: Layer.
-
-  Definition opT := linkOpT.
-  Definition State := FS.
-
-  Inductive xstep : forall T, opT T -> nat -> State -> T -> State -> Prop :=
-  | StepAdd : forall dir name target tid fs,
-    xstep (LinkAdd dir name target) tid
-      fs
-      true
-      (add_link dir target name fs)
-  | StepAllocFile : forall dir name fid tid fs,
-    file_handle_valid fs fid ->
-    file_handle_unused fs fid ->
-    xstep (LinkAllocFile dir name) tid
-      fs
-      (Some fid)
-      (add_link dir (FileNode fid) name fs)
-  | StepAllocDir : forall dir name did tid fs,
-    (~ exists pn, path_eval_root fs pn (DirNode did)) ->
-    xstep (LinkAllocDir dir name) tid
-      fs
-      (Some did)
-      (add_link dir (DirNode did) name fs)
-  | StepDel : forall dir name target tid fs,
-    xstep (LinkDel dir name target) tid
-      fs
-      true
-      (del_link dir target name fs)
-  | StepLookupAbsent : forall dir name tid fs,
-    (~ exists target, valid_link fs dir name target) ->
-    xstep (LinkLookup dir name) tid
-      fs
-      None
-      fs
-  | StepLookupFound : forall dir name target tid fs,
-    valid_link fs dir name target ->
-    xstep (LinkLookup dir name) tid
-      fs
-      (Some target)
-      fs
-  | StepList : forall dir tid fs,
-    xstep (LinkList dir) tid
-      fs
-      (Some (readdir_names fs dir))
-      fs
-  | StepGetRoot : forall tid fs,
-    xstep LinkGetRoot tid
-      fs
-      (FSRoot fs)
-      fs
-  | StepFindUnusedName : forall tid fs dir pfx name,
-    prefix pfx name = true ->
-    (~ exists target, valid_link fs dir name target) ->
-    xstep (LinkFindUnusedName dir pfx) tid
-      fs
-      name
-      fs
-  | StepRead : forall f data tid fs,
-    nth_error (FSFiles fs) f = Some data ->
-    xstep (FileRead f) tid
-      fs
-      data
-      fs
-  | StepWrite : forall f data tid fs,
-    xstep (FileWrite f data) tid
-      fs
-      tt
-      (upd_file f data fs)
-  | StepGetTID : forall tid fs,
-    xstep GetTID tid
-      fs
-      tid
-      fs.
-
-  Definition step := xstep.
-
-  Definition initP (_ : State) := True.
-
-End LinkAPI.
 
 
 Notation "x <?- p1 ; p2" := (r <- p1; match r with | None => Ret None | Some x => p2 end)
@@ -162,17 +46,17 @@ Fixpoint namei_spec (nstep : nat) (startnode : Node) (pn : Pathname) : proc _ (o
   end.
 
 Definition namei_cwd (cwd : nat) (pn : Pathname) : proc _ (option Node) :=
-  namei_spec 100 (DirNode cwd) pn.
+  namei_spec 5 (DirNode cwd) pn.
 
 Definition namei_cwd_dir (cwd : nat) (pn : Pathname) : proc _ (option nat) :=
-  r <?- namei_spec 100 (DirNode cwd) pn;
+  r <?- namei_spec 5 (DirNode cwd) pn;
   match r with
   | DirNode dirnum => Ret (Some dirnum)
   | _ => Ret None
   end.
 
 Definition namei_cwd_file (cwd : nat) (pn : Pathname) : proc _ (option nat) :=
-  r <?- namei_spec 100 (DirNode cwd) pn;
+  r <?- namei_spec 5 (DirNode cwd) pn;
   match r with
   | FileNode h => Ret (Some h)
   | _ => Ret None
