src/FS/MailServer.v
@@ -1,5 +1,6 @@
 Require Import POCS.
 Require Import FSModel.
+Require Import LinkAPI.
 Require Import FSAPI.
 Require Import MailServerAPI.
 
@@ -7,6 +8,31 @@ Import ListNotations.
 Require Import String.
 Open Scope string.
 Open Scope list.
+
+(* End-to-end layering plan:
+
+  MailServerAPI
+    |
+    | prove that our file system state matches the rep invariant
+    |
+  MailServerLinkAPI
+    |
+    | prove atomicity of our code implementing mail server opcodes;
+    | no state abstraction yet
+    |
+  MailLinkAPI
+    |
+    | prove that our code follows the [mailfs_step_allowed]
+    | protocol and maintains the invariant
+    |
+  LinkAPI
+    |
+    | adds LinkFindUnusedName, need to prove
+    |
+  BaseLinkAPI (not defined yet)
+
+*)
+
 
 Definition maildir := "mail".
 Definition tmpdir := "tmp".
@@ -20,38 +46,6 @@ Definition starts_with_tid tid (name : string) : Prop :=
   exists namesuffix,
     name = (tid_to_string tid ++ "." ++ namesuffix)%string.
 
-Axiom starts_with_tid_not_dot : forall tid name,
-    starts_with_tid tid name -> name <> ".".
-
-Axiom starts_with_tid_not_dotdot : forall tid name,
-  starts_with_tid tid name -> name <> "..".
-
-Hint Resolve starts_with_tid_not_dot.
-Hint Resolve starts_with_tid_not_dotdot.
-
-
-Axiom find_available_name : nat -> Pathname -> proc linkOpT (option string).
-
-Definition deliver (cwd : nat) (user : string) (m : message) : proc _ _ :=
-  tmpname <?- find_available_name cwd [tmpdir];
-  f <?- create cwd [tmpdir] tmpname;
-  _ <?- write cwd ([tmpdir; tmpname]) m;
-  msgname <?- find_available_name cwd ([maildir; user]);
-  _ <?- rename cwd [tmpdir] tmpname ([maildir; user]) msgname;
-  Ret (Some tt).
-
-Fixpoint read_files (cwd : nat) (dir : Pathname) (files : list string) : proc _ (option (list message)) :=
-  match files with
-  | nil => Ret (Some nil)
-  | fn :: files' =>
-    msg <?- read cwd (dir ++ [fn]);
-    others <?- read_files cwd dir files';
-    Ret (Some (msg :: others))
-  end.
-
-Definition read (cwd : nat) (user : string) : proc _ _ :=
-  filenames <?- readdir cwd ([maildir; user]);
-  read_files cwd ([maildir; user]) filenames.
 
 Inductive mailfs_step_allowed : forall T, linkOpT T -> nat -> LinkAPI.State -> Prop :=
 | MailAllowLinkAllocFile : forall dirnum name tid fs_state,
@@ -61,19 +55,24 @@ Inductive mailfs_step_allowed : forall T, linkOpT T -> nat -> LinkAPI.State -> P
 
 | MailAllowLinkLookupRoot : forall dirnum name tid fs_state,
   dirnum = FSRoot fs_state ->
+  proper_name name ->
   mailfs_step_allowed (LinkLookup dirnum name) tid fs_state
 
 | MailAllowLinkLookupTmp : forall dirnum name tid fs_state,
   starts_with_tid tid name ->
   path_eval_root fs_state [tmpdir] (DirNode dirnum) ->
+  proper_name name ->
   mailfs_step_allowed (LinkLookup dirnum name) tid fs_state
 
 | MailAllowLinkLookupMail : forall dirnum name tid fs_state,
   path_eval_root fs_state [maildir] (DirNode dirnum) ->
+  proper_name name ->
   mailfs_step_allowed (LinkLookup dirnum name) tid fs_state
 
-| MailAllowLinkLookupUser : forall dirnum name tid fs_state user,
+| MailAllowLinkLookupUser : forall dirnum name tid fs_state user f,
   path_eval_root fs_state [maildir; user] (DirNode dirnum) ->
+  proper_name name ->
+  valid_link fs_state dirnum name (FileNode f) ->
   mailfs_step_allowed (LinkLookup dirnum name) tid fs_state
 
 | MailAllowFileWrite : forall name tid fs_state f data,
@@ -85,15 +84,17 @@ Inductive mailfs_step_allowed : forall T, linkOpT T -> nat -> LinkAPI.State -> P
   path_eval_root fs_state [maildir; user; name] (FileNode f) ->
   mailfs_step_allowed (FileRead f) tid fs_state
 
-| MailAllowRenameAdd : forall dirnum name node tid fs_state user,
+| MailAllowRenameAdd : forall dirnum name f tid fs_state user,
   starts_with_tid tid name ->
   path_eval_root fs_state [maildir; user] (DirNode dirnum) ->
-  mailfs_step_allowed (LinkAdd dirnum name node) tid fs_state
+  (~ exists target, valid_link fs_state dirnum name target) ->
+  mailfs_step_allowed (LinkAdd dirnum name (FileNode f)) tid fs_state
 
-| MailAllowRenameDel : forall dirnum name node tid fs_state,
+| MailAllowRenameDel : forall dirnum name f tid fs_state,
   starts_with_tid tid name ->
   path_eval_root fs_state [tmpdir] (DirNode dirnum) ->
-  mailfs_step_allowed (LinkDel dirnum name node) tid fs_state
+  valid_link fs_state dirnum name (FileNode f) ->
+  mailfs_step_allowed (LinkDel dirnum name (FileNode f)) tid fs_state
 
 | MailAllowReaddir : forall dirnum tid fs_state user,
   path_eval_root fs_state [maildir; user] (DirNode dirnum) ->
@@ -107,14 +108,37 @@ Inductive mailfs_step_allowed : forall T, linkOpT T -> nat -> LinkAPI.State -> P
 | MailAllowFindTmp : forall dirnum tid fs_state pfx,
   starts_with_tid tid pfx ->
   path_eval_root fs_state [tmpdir] (DirNode dirnum) ->
-  mailfs_step_allowed (LinkFindUnusedName dirnum pfx) tid fs_state.
+  mailfs_step_allowed (LinkFindUnusedName dirnum pfx) tid fs_state
 
+| MailAllowGetTID : forall state tid,
+  mailfs_step_allowed GetTID tid state
+
+| MailAllowLinkGetRoot : forall state tid,
+  mailfs_step_allowed LinkGetRoot tid state.
+
+
+Definition unique_dir_pn (fs : FS) :=
+  forall pn0 pn1 d,
+    path_eval_root fs pn0 (DirNode d) ->
+    path_eval_root fs pn1 (DirNode d) ->
+    pn0 = pn1.
+
+Definition unique_pn_dir (fs : FS) :=
+  forall pn d1 d2,
+    path_eval_root fs pn (DirNode d1) ->
+    path_eval_root fs pn (DirNode d2) ->
+    d1 = d2.
 
 Definition invariant (fs : FS) :=
+  unique_dir_pn fs /\
+  unique_pn_dir fs /\
   unique_pathname_root fs [tmpdir] /\
+  proper_pathname_root fs [tmpdir] /\
   unique_pathname_root fs [maildir] /\
+  proper_pathname_root fs [maildir] /\
   forall user,
-    maybe_unique_pathname_root fs [maildir; user].
+    maybe_unique_pathname_root fs [maildir; user] /\
+    proper_pathname_root fs [maildir; user].
 
 
 Module MailLinkAPI <: Layer.
@@ -133,17 +157,792 @@ Module MailLinkAPI <: Layer.
 End MailLinkAPI.
 
 
+Module MailServerLinkAPI <: Layer.
+
+  Definition opT := mailOpT.
+  Definition State := FS.
+
+  Inductive xstep : forall T, opT T -> nat -> State -> T -> State -> Prop :=
+  | StepDeliver : forall user msg state tid userdirnum msgf name state',
+    path_eval_root state [maildir; user] (DirNode userdirnum) ->
+    starts_with_tid tid name ->
+    (~ exists target, path_eval_root state [maildir; user; name] target) ->
+    file_handle_valid state msgf ->
+    file_handle_unused state msgf ->
+    state' = create_file_write userdirnum msgf name msg state ->
+    xstep (Deliver user msg) tid
+      state
+      (Some tt)
+      state'
+  | StepRead : forall user msgs state tid,
+    (forall msg,
+      In msg msgs <->
+      exists name f,
+        path_eval_root state [maildir; user; name] (FileNode f) /\
+        nth_error (FSFiles state) f = Some msg) ->
+    xstep (Read user) tid
+      state
+      (Some msgs)
+      state
+  | StepFail : forall T (op : opT (option T)) state tid,
+    xstep op tid
+      state
+      None
+      state.
+
+  Definition step := xstep.
+
+  Definition initP (fs : State) := invariant fs.
+
+End MailServerLinkAPI.
+
+
+Axiom starts_with_tid_proper_name : forall tid name,
+  starts_with_tid tid name ->
+  proper_name name.
+
+Hint Resolve starts_with_tid_proper_name.
+
+
+Module MailAtomic <: LayerImpl MailLinkAPI MailServerLinkAPI.
+
+  Definition deliver (user : string) (m : message) : proc _ _ :=
+    cwd <- Op LinkGetRoot;
+    tid <- Op GetTID;
+    tmpname <?- find_available_name cwd [tmpdir] (tid_to_string tid);
+    f <?- create cwd [tmpdir] tmpname;
+    _ <?- write cwd ([tmpdir; tmpname]) m;
+    msgname <?- find_available_name cwd ([maildir; user]) (tid_to_string tid);
+    _ <?- rename cwd [tmpdir] tmpname ([maildir; user]) msgname;
+    Ret (Some tt).
+
+  Fixpoint read_files (cwd : nat) (dir : Pathname) (files : list string) : proc _ (option (list message)) :=
+    match files with
+    | nil => Ret (Some nil)
+    | fn :: files' =>
+      msg <?- read cwd (dir ++ [fn]);
+      others <?- read_files cwd dir files';
+      Ret (Some (msg :: others))
+    end.
+
+  Definition read (user : string) : proc _ _ :=
+    cwd <- Op LinkGetRoot;
+    filenames <?- readdir cwd ([maildir; user]);
+    read_files cwd ([maildir; user]) filenames.
+
+  Definition compile_op T (op : MailServerLinkAPI.opT T) : proc MailLinkAPI.opT T :=
+    match op with
+    | Deliver user msg => deliver user msg
+    | Read user => read user
+    end.
+
+  Ltac step_inv :=
+    match goal with
+    | H : MailLinkAPI.step _ _ _ _ _ |- _ =>
+      inversion H; clear H; subst; repeat sigT_eq
+    | H : MailServerLinkAPI.step _ _ _ _ _ |- _ =>
+      inversion H; clear H; subst; repeat sigT_eq
+    | H : mailfs_step_allowed _ _ _ |- _ =>
+      inversion H; clear H; subst; repeat sigT_eq
+    | H : LinkAPI.step _ _ _ _ _ |- _ =>
+      inversion H; clear H; subst; repeat sigT_eq
+    end.
+
+  Hint Extern 1 (MailLinkAPI.step _ _ _ _ _) => econstructor.
+  Hint Extern 1 (MailServerLinkAPI.step _ _ _ _ _) => econstructor.
+  Hint Extern 1 (LinkAPI.step _ _ _ _ _) => econstructor.
+  Hint Constructors mailfs_step_allowed.
+
+
+  Lemma link_get_root_right_mover :
+    right_mover MailLinkAPI.step LinkGetRoot.
+  Proof.
+    unfold right_mover; intros.
+    inversion H0; clear H0.
+    inversion H2; clear H2; repeat sigT_eq.
+    eexists; split; eauto.
+    repeat ( step_inv; intuition idtac ).
+    all: eauto.
+  Qed.
+
+  Lemma get_tid_right_mover :
+    right_mover MailLinkAPI.step GetTID.
+  Proof.
+    unfold right_mover; intros.
+    inversion H0; clear H0.
+    inversion H2; clear H2; repeat sigT_eq.
+    eexists; split; eauto.
+    repeat ( step_inv; intuition idtac ).
+    all: eauto.
+  Qed.
+
+  Lemma valid_link_add_link : forall fs dirnum name target dirnum0 name0 target0,
+    valid_link (add_link dirnum0 target0 name0 fs) dirnum name target ->
+    dirnum <> dirnum0 ->
+    proper_name name ->
+    proper_name name0 ->
+    valid_link fs dirnum name target.
+  Proof.
+  Admitted.
+
+  Lemma valid_link_add_link' : forall fs dirnum name target dirnum0 name0 target0,
+    valid_link fs dirnum name target ->
+    dirnum <> dirnum0 ->
+    proper_name name ->
+    proper_name name0 ->
+    valid_link (add_link dirnum0 target0 name0 fs) dirnum name target.
+  Proof.
+  Admitted.
+
+  Lemma valid_link_del_link : forall fs dirnum name target dirnum0 name0 target0,
+    valid_link (del_link dirnum0 target0 name0 fs) dirnum name target ->
+    dirnum <> dirnum0 ->
+    proper_name name ->
+    proper_name name0 ->
+    valid_link fs dirnum name target.
+  Proof.
+  Admitted.
+
+  Lemma valid_link_del_link' : forall fs dirnum name target dirnum0 name0 target0,
+    valid_link fs dirnum name target ->
+    dirnum <> dirnum0 ->
+    proper_name name ->
+    proper_name name0 ->
+    valid_link (del_link dirnum0 target0 name0 fs) dirnum name target.
+  Proof.
+  Admitted.
+
+  Lemma valid_link_upd_file : forall fs dirnum name target f data,
+    valid_link (upd_file f data fs) dirnum name target ->
+    proper_name name ->
+    valid_link fs dirnum name target.
+  Proof.
+  Admitted.
+
+  Lemma valid_link_upd_file' : forall fs dirnum name target f data,
+    valid_link fs dirnum name target ->
+    proper_name name ->
+    valid_link (upd_file f data fs) dirnum name target.
+  Proof.
+  Admitted.
+
+  Hint Extern 1 (valid_link ?fs ?dir ?name ?target) =>
+    match goal with
+    | H : valid_link (upd_file _ _ fs) dir name _ |- _ =>
+      eapply valid_link_upd_file
+    end.
+
+  Hint Extern 1 (valid_link ?fs ?dir ?name ?target) =>
+    match goal with
+    | H : valid_link (del_link _ _ _ fs) dir name _ |- _ =>
+      eapply valid_link_del_link
+    end.
+
+  Hint Extern 1 (valid_link ?fs ?dir ?name ?target) =>
+    match goal with
+    | H : valid_link (add_link _ _ _ fs) dir name _ |- _ =>
+      eapply valid_link_add_link
+    end.
+
+  Hint Resolve valid_link_add_link'.
+  Hint Resolve valid_link_del_link'.
+  Hint Resolve valid_link_upd_file'.
+
+  Lemma valid_link_add_link_ne_name : forall fs dirnum name target dirnum0 name0 target0,
+    valid_link (add_link dirnum0 target0 name0 fs) dirnum name target ->
+    name <> name0 ->
+    proper_name name ->
+    proper_name name0 ->
+    valid_link fs dirnum name target.
+  Proof.
+  Admitted.
+
+  Lemma valid_link_del_link_ne_name : forall fs dirnum name target dirnum0 name0 target0,
+    valid_link (del_link dirnum0 target0 name0 fs) dirnum name target ->
+    name <> name0 ->
+    proper_name name ->
+    proper_name name0 ->
+    valid_link fs dirnum name target.
+  Proof.
+  Admitted.
+
+  Lemma valid_link_add_link_ne_name' : forall fs dirnum name target dirnum0 name0 target0,
+    valid_link fs dirnum name target ->
+    name <> name0 ->
+    proper_name name ->
+    proper_name name0 ->
+    valid_link (add_link dirnum0 target0 name0 fs) dirnum name target.
+  Proof.
+  Admitted.
+
+  Lemma valid_link_del_link_ne_name' : forall fs dirnum name target dirnum0 name0 target0,
+    valid_link fs dirnum name target ->
+    name <> name0 ->
+    proper_name name ->
+    proper_name name0 ->
+    valid_link (del_link dirnum0 target0 name0 fs) dirnum name target.
+  Proof.
+  Admitted.
+
+  Hint Extern 1 (valid_link ?fs ?dir ?name ?target) =>
+    match goal with
+    | H : valid_link (add_link _ _ _ fs) dir name _ |- _ =>
+      eapply valid_link_add_link_ne_name
+    end.
+
+  Hint Extern 1 (valid_link ?fs ?dir ?name ?target) =>
+    match goal with
+    | H : valid_link (del_link _ _ _ fs) dir name _ |- _ =>
+      eapply valid_link_del_link_ne_name
+    end.
+
+  Hint Resolve valid_link_add_link_ne_name'.
+  Hint Resolve valid_link_del_link_ne_name'.
+
+  Axiom starts_with_tid_ne : forall tid0 tid1 name0 name1,
+    starts_with_tid tid0 name0 ->
+    starts_with_tid tid1 name1 ->
+    tid0 <> tid1 ->
+    name0 <> name1.
+
+  Hint Resolve starts_with_tid_ne.
+
+
+  Lemma path_eval_root_add_link_file : forall fs pn dirnum dirnum0 f name0,
+    path_eval_root fs pn (DirNode dirnum) ->
+    path_eval_root (add_link dirnum0 (FileNode f) name0 fs) pn (DirNode dirnum).
+  Admitted.
+
+  Lemma path_eval_root_del_link_file : forall fs pn dirnum dirnum0 f name0,
+    path_eval_root fs pn (DirNode dirnum) ->
+    path_eval_root (del_link dirnum0 (FileNode f) name0 fs) pn (DirNode dirnum).
+  Admitted.
+
+  Lemma path_eval_root_upd_file : forall fs pn dirnum f data,
+    path_eval_root fs pn (DirNode dirnum) ->
+    path_eval_root (upd_file f data fs) pn (DirNode dirnum).
+  Admitted.
+
+  Hint Resolve path_eval_root_add_link_file.
+  Hint Resolve path_eval_root_del_link_file.
+  Hint Resolve path_eval_root_upd_file.
+
+
+  Lemma proper_pathname_distinct : forall s pn d0 d1,
+    path_evaluates s (DirNode d0) pn (DirNode d1) ->
+    proper_pathname s d0 pn ->
+    pn <> nil ->
+    d0 <> d1.
+  Admitted.
+
+  Lemma proper_pathname_distinct_root : forall s pn d1,
+    path_eval_root s pn (DirNode d1) ->
+    proper_pathname_root s pn ->
+    pn <> nil ->
+    FSRoot s <> d1.
+  Proof.
+    unfold path_eval_root; intros.
+    eapply proper_pathname_distinct; eauto.
+  Qed.
+
+  Lemma proper_pathname_distinct_tmpdir : forall s d1,
+    path_eval_root s [tmpdir] (DirNode d1) ->
+    invariant s ->
+    FSRoot s <> d1.
+  Proof.
+    unfold invariant; intuition idtac.
+    eapply proper_pathname_distinct_root; eauto.
+    congruence.
+  Qed.
+
+  Lemma proper_pathname_distinct_maildir : forall s d1,
+    path_eval_root s [maildir] (DirNode d1) ->
+    invariant s ->
+    FSRoot s <> d1.
+  Proof.
+    unfold invariant; intuition idtac.
+    eapply proper_pathname_distinct_root; eauto.
+    congruence.
+  Qed.
+
+  Lemma proper_pathname_distinct_userdir : forall s user d1,
+    path_eval_root s [maildir; user] (DirNode d1) ->
+    invariant s ->
+    FSRoot s <> d1.
+  Proof.
+    unfold invariant; intuition idtac.
+    eapply proper_pathname_distinct_root; eauto.
+    edestruct H8; eauto.
+    congruence.
+  Qed.
+
+  Hint Resolve proper_pathname_distinct_tmpdir.
+  Hint Resolve proper_pathname_distinct_maildir.
+  Hint Resolve proper_pathname_distinct_userdir.
+
+
+  Lemma unique_dir_pn_ne : forall fs pn1 pn2 d1 d2,
+    invariant fs ->
+    path_eval_root fs pn1 (DirNode d1) ->
+    path_eval_root fs pn2 (DirNode d2) ->
+    pn1 <> pn2 ->
+    d1 <> d2.
+  Proof.
+    unfold invariant; intuition idtac; subst.
+    eapply H4 in H0.
+    eapply H0 in H1.
+    congruence.
+  Qed.
+
+  Lemma unique_dir_pn_eq : forall fs pn d1 d2,
+    invariant fs ->
+    path_eval_root fs pn (DirNode d1) ->
+    path_eval_root fs pn (DirNode d2) ->
+    d1 = d2.
+  Proof.
+    unfold invariant; intuition idtac; subst.
+    eapply H in H0.
+    eapply H0 in H1.
+    congruence.
+  Qed.
+
+  Hint Resolve unique_dir_pn_ne.
+  Hint Resolve unique_dir_pn_eq.
+
+  Lemma maildir_ne_tmpdir : [maildir] <> [tmpdir].
+  Proof.
+    intro.
+    inversion H.
+  Qed.
+
+  Lemma maildir_ne_maildir_user : forall user,
+    [maildir] <> [maildir; user].
+  Proof.
+    congruence.
+  Qed.
+
+  Lemma tmpdir_ne_maildir_user : forall user,
+    [tmpdir] <> [maildir; user].
+  Proof.
+    congruence.
+  Qed.
+
+  Lemma maildir_user_ne_maildir_user : forall user1 user2,
+    user1 <> user2 ->
+    [maildir; user1] <> [maildir; user2].
+  Proof.
+    congruence.
+  Qed.
+
+  Hint Resolve maildir_ne_tmpdir.
+  Hint Resolve maildir_ne_maildir_user.
+  Hint Resolve tmpdir_ne_maildir_user.
+  Hint Resolve maildir_user_ne_maildir_user.
+
+
+  Lemma link_lookup_right_mover : forall dirnum name,
+    right_mover MailLinkAPI.step (LinkLookup dirnum name).
+  Proof.
+    unfold right_mover; intros.
+    exists s1.
+    inversion H0; clear H0; intuition idtac.
+    - inversion H2; clear H2; subst; repeat sigT_eq; eauto.
+    - inversion H0; clear H0; subst; repeat sigT_eq.
+      + (* MailAllowLinkLookupRoot *)
+        inversion H2; clear H2; subst; repeat sigT_eq.
+        * (* lookup failed *)
+          repeat ( step_inv; intuition idtac ).
+          par: eauto 10.
+
+         -- econstructor; eauto.
+            econstructor.
+            contradict H10; deex. eauto.
+         -- econstructor; eauto.
+            econstructor.
+            contradict H10; deex. eauto.
+         -- econstructor; eauto.
+            econstructor.
+            contradict H10; deex. eauto.
+         -- econstructor; eauto.
+            econstructor.
+            contradict H10; deex. eauto.
+
+        * (* lookup succeeded *)
+          repeat ( step_inv; intuition idtac ).
+          par: eauto 10.
+
+      + (* MailAllowLinkLookupTmp *)
+        inversion H2; clear H2; subst; repeat sigT_eq.
+        * (* lookup failed *)
+          repeat ( step_inv; intuition idtac ).
+          all: eauto 6.
+
+         -- econstructor; eauto.
+            econstructor.
+            contradict H12; deex. eauto.
+
+         -- econstructor; eauto.
+            econstructor.
+            contradict H12; deex. eauto.
+
+         -- econstructor; eauto.
+            econstructor.
+            contradict H12; deex. eauto.
+
+         -- econstructor; eauto.
+            econstructor.
+            contradict H12; deex. eauto.
+
+        * (* lookup succeeded *)
+          repeat ( step_inv; intuition idtac ).
+          par: eauto 10.
+
+      + (* MailAllowLinkLookupMail *)
+        inversion H2; clear H2; subst; repeat sigT_eq.
+        * (* lookup failed *)
+          repeat ( step_inv; intuition idtac ).
+          all: eauto 6.
+
+         -- econstructor; eauto.
+            econstructor.
+            contradict H11; deex. eauto.
+
+         -- econstructor; eauto.
+            econstructor.
+            contradict H11; deex. eauto.
+
+         -- econstructor; eauto.
+            econstructor.
+            contradict H11; deex. eauto.
+
+         -- econstructor; eauto.
+            econstructor.
+            contradict H11; deex. eauto.
+
+        * (* lookup succeeded *)
+          repeat ( step_inv; intuition idtac ).
+          par: eauto 10.
+
+      + (* MailAllowLinkLookupUser *)
+        inversion H2; clear H2; subst; repeat sigT_eq.
+        * (* lookup failed *)
+          repeat ( step_inv; intuition idtac ).
+          all: eauto 15.
+
+        * (* lookup succeeded *)
+          repeat ( step_inv; intuition idtac ).
+          par: eauto 15.
+
+          destruct (user0 == user); subst.
+         -- assert (dirnum0 = dirnum) by ( eapply unique_dir_pn_eq; eauto ).
+            subst.
+
+            assert (name <> name0).
+            contradict H17; subst; eauto.
+            eauto 20.
+
+         -- assert (dirnum0 <> dirnum) by ( eapply unique_dir_pn_ne; eauto ).
+            eauto 20.
+  Qed.
+
+  Ltac atomic_exec_inv_with_options :=
+    match goal with
+    | H : atomic_exec _ (match ?r with _ => _ end) _ _ _ _ _ |- _ =>
+      destruct r
+    | H : atomic_exec _ _ _ _ _ _ _ |- _ =>
+      idtac H;
+      inversion H; clear H; subst; repeat maybe_proc_inv
+    | H : Some _ = Some _ |- _ =>
+      inversion H; clear H; subst
+    end;
+    autorewrite with t in *;
+    try congruence.
+
+  Ltac apply_in_atomic_exec H :=
+    match goal with
+    | Ha : atomic_exec _ _ _ _ _ _ _ |- _ =>
+      apply H in Ha
+    end.
+
+  Lemma namei_spec_path_evaluates_some :
+    forall n fs cwd pn tid r fs' evs,
+    atomic_exec MailLinkAPI.step (namei_spec n cwd pn) tid fs (Some r) fs' evs ->
+      evs = [] /\
+      fs' = fs /\
+      path_evaluates fs cwd pn r.
+  Proof.
+    induction n; intros; simpl in *.
+    - repeat atomic_exec_inv_with_options.
+    - repeat ( apply_in_atomic_exec IHn ||
+               atomic_exec_inv_with_options ||
+               step_inv ||
+               congruence ).
+      eauto.
+      all: intuition idtac; subst; simpl; try congruence.
+      all: eauto with model.
+      inversion H5; subst.
+      eauto.
+  Qed.
+
+  Lemma namei_spec_path_evaluates_none :
+    forall n fs cwd pn tid fs' evs,
+    atomic_exec MailLinkAPI.step (namei_spec n cwd pn) tid fs None fs' evs ->
+      evs = [] /\
+      fs' = fs.
+  Proof.
+    induction n; intros; simpl in *.
+    - repeat atomic_exec_inv_with_options.
+      eauto.
+    - repeat ( apply_in_atomic_exec IHn ||
+               apply_in_atomic_exec namei_spec_path_evaluates_some ||
+               atomic_exec_inv_with_options ||
+               step_inv ||
+               congruence ).
+      eauto.
+      all: intuition idtac; subst; simpl; try congruence.
+  Qed.
+
+  Opaque namei_spec.
+
+  Lemma namei_cwd_dir_path_evaluates_some :
+    forall fs cwd pn tid r fs' evs,
+    atomic_exec MailLinkAPI.step (namei_cwd_dir cwd pn) tid fs (Some r) fs' evs ->
+      evs = [] /\
+      fs' = fs /\
+      path_evaluates fs (DirNode cwd) pn (DirNode r).
+  Proof.
+    intros.
+    repeat ( apply_in_atomic_exec namei_spec_path_evaluates_some ||
+             apply_in_atomic_exec namei_spec_path_evaluates_none ||
+             atomic_exec_inv_with_options ||
+             step_inv ||
+             congruence ).
+    rewrite app_nil_r.
+    intuition eauto.
+  Qed.
+
+  Lemma namei_cwd_dir_path_evaluates_none :
+    forall fs cwd pn tid fs' evs,
+    atomic_exec MailLinkAPI.step (namei_cwd_dir cwd pn) tid fs None fs' evs ->
+      evs = [] /\
+      fs' = fs.
+  Proof.
+    intros.
+    repeat ( apply_in_atomic_exec namei_spec_path_evaluates_some ||
+             apply_in_atomic_exec namei_spec_path_evaluates_none ||
+             atomic_exec_inv_with_options ||
+             step_inv ||
+             congruence ).
+    all: rewrite app_nil_r.
+    all: intuition eauto.
+  Qed.
+
+  Lemma namei_cwd_file_path_evaluates_some :
+    forall fs cwd pn tid r fs' evs,
+    atomic_exec MailLinkAPI.step (namei_cwd_file cwd pn) tid fs (Some r) fs' evs ->
+      evs = [] /\
+      fs' = fs /\
+      path_evaluates fs (DirNode cwd) pn (FileNode r).
+  Proof.
+    intros.
+    repeat ( apply_in_atomic_exec namei_spec_path_evaluates_some ||
+             apply_in_atomic_exec namei_spec_path_evaluates_none ||
+             atomic_exec_inv_with_options ||
+             step_inv ||
+             congruence ).
+    rewrite app_nil_r.
+    intuition eauto.
+  Qed.
+
+  Lemma namei_cwd_file_path_evaluates_none :
+    forall fs cwd pn tid fs' evs,
+    atomic_exec MailLinkAPI.step (namei_cwd_file cwd pn) tid fs None fs' evs ->
+      evs = [] /\
+      fs' = fs.
+  Proof.
+    intros.
+    repeat ( apply_in_atomic_exec namei_spec_path_evaluates_some ||
+             apply_in_atomic_exec namei_spec_path_evaluates_none ||
+             atomic_exec_inv_with_options ||
+             step_inv ||
+             congruence ).
+    all: rewrite app_nil_r.
+    all: intuition eauto.
+  Qed.
+
+  Lemma read_files_ok :
+    forall files fs cwd dir tid fs' evs r,
+    atomic_exec MailLinkAPI.step (read_files cwd dir files) tid fs r fs' evs ->
+      evs = [] /\
+      fs' = fs /\
+      match r with
+      | Some msgs =>
+        Forall2 (fun fn msg =>
+          exists f,
+            path_evaluates fs (DirNode cwd) (dir ++ [fn]) (FileNode f) /\
+            nth_error (FSFiles fs) f = Some msg) files msgs
+      | None => True
+      end.
+  Proof.
+    induction files; intros; simpl in *.
+    - repeat atomic_exec_inv_with_options.
+      eauto.
+    - repeat ( unfold message in * ||
+               apply_in_atomic_exec IHfiles ||
+               apply_in_atomic_exec namei_spec_path_evaluates_some ||
+               apply_in_atomic_exec namei_spec_path_evaluates_none ||
+               atomic_exec_inv_with_options ||
+               step_inv ||
+               congruence ).
+      all: intuition subst; eauto.
+  Qed.
+
+  Theorem my_compile_correct :
+    compile_correct compile_op MailLinkAPI.step MailServerLinkAPI.step.
+  Proof.
+    unfold compile_correct; intros.
+    destruct op.
+
+    - do 40 ( step_inv ||
+               rewrite app_nil_r ||
+               rewrite app_nil_l ||
+               solve [ intuition subst; eauto ] ||
+               apply_in_atomic_exec namei_cwd_dir_path_evaluates_some ||
+               apply_in_atomic_exec namei_cwd_dir_path_evaluates_none ||
+               apply_in_atomic_exec namei_cwd_file_path_evaluates_some ||
+               apply_in_atomic_exec namei_cwd_file_path_evaluates_none ||
+               apply_in_atomic_exec namei_spec_path_evaluates_some ||
+               apply_in_atomic_exec namei_spec_path_evaluates_none ||
+               atomic_exec_inv_with_options ).
+
+do 40 ( step_inv ||
+               rewrite app_nil_r ||
+               rewrite app_nil_l ||
+               solve [ intuition subst; eauto ] ||
+               apply_in_atomic_exec namei_cwd_dir_path_evaluates_some ||
+               apply_in_atomic_exec namei_cwd_dir_path_evaluates_none ||
+               apply_in_atomic_exec namei_cwd_file_path_evaluates_some ||
+               apply_in_atomic_exec namei_cwd_file_path_evaluates_none ||
+               apply_in_atomic_exec namei_spec_path_evaluates_some ||
+               apply_in_atomic_exec namei_spec_path_evaluates_none ||
+               atomic_exec_inv_with_options ).
+
+repeat ( step_inv ||
+               rewrite app_nil_r ||
+               rewrite app_nil_l ||
+               solve [ intuition subst; eauto ] ||
+               apply_in_atomic_exec namei_cwd_dir_path_evaluates_some ||
+               apply_in_atomic_exec namei_cwd_dir_path_evaluates_none ||
+               apply_in_atomic_exec namei_cwd_file_path_evaluates_some ||
+               apply_in_atomic_exec namei_cwd_file_path_evaluates_none ||
+               apply_in_atomic_exec namei_spec_path_evaluates_some ||
+               apply_in_atomic_exec namei_spec_path_evaluates_none ||
+               atomic_exec_inv_with_options ).
+
+intuition subst. eauto.
+replace n1 with n2 in *.
+exfalso; eauto.
+replace (FSRoot s2) with (FSRoot (upd_file n3 m (add_link n4 (FileNode n) v3 s2))) in *.
+eapply unique_dir_pn_eq.
+2: unfold path_eval_root; eauto.
+2: unfold path_eval_root; eauto.
+eauto.
+reflexivity.
+
+
+
+repeat ( step_inv ||
+               rewrite app_nil_r ||
+               rewrite app_nil_l ||
+               solve [ intuition subst; eauto ] ||
+               apply_in_atomic_exec namei_cwd_dir_path_evaluates_some ||
+               apply_in_atomic_exec namei_cwd_dir_path_evaluates_none ||
+               apply_in_atomic_exec namei_cwd_file_path_evaluates_some ||
+               apply_in_atomic_exec namei_cwd_file_path_evaluates_none ||
+               apply_in_atomic_exec namei_spec_path_evaluates_some ||
+               apply_in_atomic_exec namei_spec_path_evaluates_none ||
+               atomic_exec_inv_with_options ).
+
+repeat ( step_inv ||
+               rewrite app_nil_r ||
+               rewrite app_nil_l ||
+               solve [ intuition subst; eauto ] ||
+               apply_in_atomic_exec namei_cwd_dir_path_evaluates_some ||
+               apply_in_atomic_exec namei_cwd_dir_path_evaluates_none ||
+               apply_in_atomic_exec namei_cwd_file_path_evaluates_some ||
+               apply_in_atomic_exec namei_cwd_file_path_evaluates_none ||
+               apply_in_atomic_exec namei_spec_path_evaluates_some ||
+               apply_in_atomic_exec namei_spec_path_evaluates_none ||
+               atomic_exec_inv_with_options ).
+
+intuition subst. eauto.
+econstructor.
+admit.
+admit.
+admit.
+eauto.
+eauto.
+unfold create_file_write.
+admit.
+
+Search user.
+Search path_evaluates add_link.
+exfalso; eauto.
+replace (FSRoot s2) with (FSRoot (upd_file n3 m (add_link n4 (FileNode n) v3 s2))) in *.
+eapply unique_dir_pn_eq.
+2: unfold path_eval_root; eauto.
+2: unfold path_eval_root; eauto.
+eauto.
+reflexivity.
+
+
+econstructor.
+Search path_evaluates user.
+
+
+Search n2.
+
+Focus 12.
+
+repeat ( step_inv ||
+               rewrite app_nil_r ||
+               rewrite app_nil_l ||
+               solve [ intuition subst; eauto ] ||
+               apply_in_atomic_exec namei_spec_path_evaluates_some ||
+               apply_in_atomic_exec namei_spec_path_evaluates_none ||
+               atomic_exec_inv_with_options ).
+*)
+    - repeat ( step_inv ||
+               rewrite app_nil_r ||
+               rewrite app_nil_l ||
+               solve [ intuition subst; eauto ] ||
+               apply_in_atomic_exec read_files_ok ||
+               apply_in_atomic_exec namei_spec_path_evaluates_some ||
+               apply_in_atomic_exec namei_spec_path_evaluates_none ||
+               atomic_exec_inv_with_options ).
+
+      intuition subst; eauto.
+      destruct v.
+      + econstructor; intros.
+        split; intros.
+        * generalize dependent (readdir_names s1 dirnum).
+          induction l; intros. inversion H.
+          inversion H8; clear H8. deex.
+          inversion H; clear H; subst.
+         -- do 2 eexists. unfold path_eval_root. simpl in *.
+            eauto.
+         -- eauto.
+        * repeat deex.
+          admit.
+      + eauto.
+  Admitted.
+
 
 Hint Constructors mailfs_step_allowed.
 
 Axiom tmpdir_not_maildir : forall user, tmpdir = (maildir ++ [user])%list -> False.
 Hint Resolve tmpdir_not_maildir.
 
-Axiom starts_with_tid_ne : forall tid0 tid1 name0 name1,
-  tid0 <> tid1 ->
-  starts_with_tid tid0 name0 ->
-  starts_with_tid tid1 name1 ->
-  name0 <> name1.
 
 Hint Resolve starts_with_tid_ne.
 
