src/FS/LinkAPI.v
@@ -1,0 +1,116 @@
+Require Import POCS.
+Require Import String.
+Require Import Equalities.
+Require Import MSets.MSetWeakList.
+Require Import Relations.Relation_Operators.
+Require Import RelationClasses.
+Require Import Morphisms.
+Require Import Sumbool.
+Require Import FSModel.
+
+Import ListNotations.
+Open Scope string.
+
+
+(** Opcodes *)
+
+Inductive linkOpT : Type -> Type :=
+| LinkAdd (dir : nat) (name : string) (target : Node) : linkOpT bool
+| LinkAllocFile (dir : nat) (name : string) : linkOpT (option nat)
+| LinkAllocDir (dir : nat) (name : string) : linkOpT (option nat)
+| LinkDel (dir : nat) (name : string) (target : Node) : linkOpT bool
+| LinkLookup (dir : nat) (name : string) : linkOpT (option Node)
+| LinkList (dir : nat) : linkOpT (option (list string))
+| LinkGetRoot : linkOpT nat
+| LinkFindUnusedName (dir : nat) (prefix : string) : linkOpT string
+| FileRead (f : nat) : linkOpT string
+| FileWrite (f : nat) (data : string) : linkOpT unit
+| GetTID : linkOpT nat.
+
+
+Inductive stat_result :=
+| StatFile
+| StatDir.
+
+
+Module LinkAPI <: Layer.
+
+  Definition opT := linkOpT.
+  Definition State := FS.
+
+  Inductive xstep : forall T, opT T -> nat -> State -> T -> State -> Prop :=
+  | StepAdd : forall dir name target tid fs,
+    xstep (LinkAdd dir name target) tid
+      fs
+      true
+      (add_link dir target name fs)
+  | StepAllocFile : forall dir name fid tid fs,
+    file_handle_valid fs fid ->
+    file_handle_unused fs fid ->
+    xstep (LinkAllocFile dir name) tid
+      fs
+      (Some fid)
+      (add_link dir (FileNode fid) name fs)
+  | StepAllocDir : forall dir name did tid fs,
+    (~ exists pn, path_eval_root fs pn (DirNode did)) ->
+    xstep (LinkAllocDir dir name) tid
+      fs
+      (Some did)
+      (add_link dir (DirNode did) name fs)
+  | StepDel : forall dir name target tid fs,
+    xstep (LinkDel dir name target) tid
+      fs
+      true
+      (del_link dir target name fs)
+  | StepLookupAbsent : forall dir name tid fs,
+    (~ exists target, valid_link fs dir name target) ->
+    xstep (LinkLookup dir name) tid
+      fs
+      None
+      fs
+  | StepLookupFound : forall dir name target tid fs,
+    valid_link fs dir name target ->
+    xstep (LinkLookup dir name) tid
+      fs
+      (Some target)
+      fs
+  | StepList : forall dir tid fs,
+    xstep (LinkList dir) tid
+      fs
+      (Some (readdir_names fs dir))
+      fs
+  | StepGetRoot : forall tid fs r,
+    r = FSRoot fs ->
+    xstep LinkGetRoot tid
+      fs
+      r
+      fs
+  | StepFindUnusedName : forall tid fs dir pfx name,
+    prefix pfx name = true ->
+    (~ exists target, valid_link fs dir name target) ->
+    xstep (LinkFindUnusedName dir pfx) tid
+      fs
+      name
+      fs
+  | StepRead : forall f data tid fs,
+    nth_error (FSFiles fs) f = Some data ->
+    xstep (FileRead f) tid
+      fs
+      data
+      fs
+  | StepWrite : forall f data tid fs,
+    xstep (FileWrite f data) tid
+      fs
+      tt
+      (upd_file f data fs)
+  | StepGetTID : forall tid fs,
+    xstep GetTID tid
+      fs
+      tid
+      fs.
+
+  Definition step := xstep.
+
+  Definition initP (_ : State) := True.
+
+End LinkAPI.
