src/POCS.v
@@ -34,3 +34,4 @@ Require Export Spec.Equiv.
 Require Export Spec.Compile.
 Require Export Spec.Abstraction.
 Require Export Spec.Modules.
+Require Export Spec.Movers.
